src/PermCacheLemmas.v
@@ -6,7 +6,6 @@ Require Import Array.
 Require Import Pred.
 Require Import WordAuto.
 Require Import Omega.
-Require Import AsyncDisk.
 Require Import ListUtils.
 Require Import OrderedTypeEx.
 Require Import Arith.
@@ -14,8 +13,8 @@ Require Import MapUtils.
 Require Import MemPred.
 Require Import ListPred.
 Require Import FunctionalExtensionality.
-Require Export PermCacheDef.
 Require Import ADestructPair DestructVarname.
+Require Export PermCacheDef.
 
 Import AddrMap.
 Import Map.
@@ -36,6 +35,52 @@ Proof.
   apply elements_2 in A; auto.
 Qed.
 
+Theorem sync_invariant_cachepred :
+  forall cache a vs bm,
+    sync_invariant (cachepred cache bm a vs).
+Proof.
+  unfold cachepred; intros.
+  destruct (Map.find a cache); eauto.
+  destruct p; destruct b; eauto.
+Qed.
+
+Theorem sync_invariant_synpred :
+  forall cache bm a vs,
+    sync_invariant (synpred cache bm a vs).
+Proof.
+  unfold synpred; intros.
+  destruct (Map.find a cache); eauto.
+  destruct p; destruct b; eauto.
+Qed.
+
+Hint Resolve sync_invariant_cachepred sync_invariant_synpred.
+
+Theorem sync_invariant_rep :
+  forall (cs: cachestate) m bm,
+    sync_invariant (rep cs m bm).
+Proof.
+  unfold rep; intros; eauto.
+Qed.
+
+Hint Resolve sync_invariant_rep.
+
+Theorem sync_invariant_synrep' :
+  forall cs m bm,
+  sync_invariant (synrep' cs m bm).
+Proof.
+  unfold synrep'; eauto.
+Qed.
+
+Hint Resolve sync_invariant_synrep'.
+
+Theorem sync_invariant_synrep :
+  forall cs mbase m bm,
+    sync_invariant (synrep cs mbase m bm).
+Proof.
+  unfold synrep; eauto.
+Qed.
+
+Hint Resolve sync_invariant_synrep.
 
 
   Lemma cachepred_remove_invariant : forall a a' v cache bm,
@@ -52,9 +97,24 @@ Qed.
     rewrite MapFacts.add_neq_o; auto.
   Qed.
 
+    Lemma synpred_remove_invariant : forall a a' v cache bm,
+    a <> a' -> synpred cache bm a v =p=> synpred (Map.remove a' cache) bm a v.
+  Proof.
+    unfold synpred; intros.
+    rewrite MapFacts.remove_neq_o; auto.
+  Qed.
+
+  Lemma synpred_add_invariant : forall a a' v v' cache bm,
+    a <> a' -> synpred cache bm a v =p=> synpred (Map.add a' v' cache) bm a v.
+  Proof.
+    unfold synpred; intros.
+    rewrite MapFacts.add_neq_o; auto.
+  Qed.
+
+
 Lemma mem_pred_cachepred_remove_absorb : forall csmap d a w bm,
     d a = Some w ->
-    mem_pred (HighAEQ:= addr_eq_dec) (cachepred csmap bm) (mem_except d a) * a |-> w =p=>
+    mem_pred (HighAEQ:= addr_eq_dec) (cachepred csmap bm) (mem_except d a) * a |+> w =p=>
     mem_pred (HighAEQ:= addr_eq_dec) (cachepred (remove a csmap) bm) d.
   Proof.
     intros.
@@ -69,9 +129,9 @@ Lemma mem_pred_cachepred_remove_absorb : forall csmap d a w bm,
 
 Lemma addr_clean_cachepred_remove_none :
   forall cs a d bm,
-    find a (HCSMap cs) = None ->
-    mem_pred (HighAEQ:= addr_eq_dec) (cachepred (HCSMap cs) bm) d =p=>
-      mem_pred (HighAEQ:= addr_eq_dec) (cachepred (remove a (HCSMap cs)) bm) d.
+    find a (CSMap cs) = None ->
+    mem_pred (HighAEQ:= addr_eq_dec) (cachepred (CSMap cs) bm) d =p=>
+      mem_pred (HighAEQ:= addr_eq_dec) (cachepred (remove a (CSMap cs)) bm) d.
 Proof.
   intros.
   eapply mem_pred_pimpl; intros.
@@ -83,13 +143,13 @@ Qed.
 
 Lemma addr_clean_cachepred_remove :
   forall cs a d F vs bm,
-    addr_clean (HCSMap cs) a ->
-    (F * a |-> vs)%pred d ->
-    mem_pred (HighAEQ:= addr_eq_dec) (cachepred (HCSMap cs) bm) d =p=>
-      mem_pred (HighAEQ:= addr_eq_dec) (cachepred (remove a (HCSMap cs)) bm) d.
+    addr_clean (CSMap cs) a ->
+    (F * a |+> vs)%pred d ->
+    mem_pred (HighAEQ:= addr_eq_dec) (cachepred (CSMap cs) bm) d =p=>
+      mem_pred (HighAEQ:= addr_eq_dec) (cachepred (remove a (CSMap cs)) bm) d.
   Proof.
     unfold addr_clean; intros.
-    apply ptsto_valid' in H0; cleanup.
+    apply ptsto_subset_valid' in H0; cleanup.
     destruct H; cleanup.
     - rewrite mem_pred_extract with (a := a) by eauto.
       unfold cachepred at 2; rewrite H.
@@ -103,27 +163,28 @@ Lemma addr_clean_cachepred_remove :
       eapply mem_pred_cachepred_remove_absorb; eauto.
   Qed.
 
-  Lemma addr_valid_ptsto_exists:
+  Lemma addr_valid_ptsto_subset:
       forall a b cs d,
-        addr_valid d (HCSMap cs) ->
-        find a (HCSMap cs) = Some b ->
-        exists F tb, (sep_star (AEQ:=addr_eq_dec) F (a|->tb))%pred d.
+        addr_valid d (CSMap cs) ->
+        find a (CSMap cs) = Some b ->
+        exists F tb, (sep_star (AEQ:=addr_eq_dec) F (a|+>tb))%pred d.
     Proof.
       unfold rep, addr_valid; intros.
       destruct_lift H.
-      assert (A: find a (HCSMap cs) <> None ).
+      assert (A: find a (CSMap cs) <> None ).
       intuition; congruence.
       apply MapFacts.in_find_iff in A.
       specialize (H _ A).
       destruct (d a) eqn:D; try congruence.
       do 2 eexists.
+      erewrite <- ptsto_pimpl_ptsto_subset.
       apply any_sep_star_ptsto; eauto.
     Qed.
 
   Lemma size_valid_remove : forall cs a,
     size_valid cs ->
-    Map.In a (HCSMap cs) ->
-    size_valid (mk_cs (Map.remove a (HCSMap cs)) (HCSMaxCount cs) (HCSCount cs - 1) (HCSEvict cs)).
+    Map.In a (CSMap cs) ->
+    size_valid (mk_cs (Map.remove a (CSMap cs)) (CSMaxCount cs) (CSCount cs - 1) (CSEvict cs)).
   Proof.
     unfold size_valid in *; intuition simpl.
     rewrite map_remove_cardinal by eauto; congruence.
@@ -134,8 +195,8 @@ Lemma addr_clean_cachepred_remove :
 
   Lemma size_valid_remove_notin : forall cs a,
     size_valid cs ->
-    ~ Map.In a (HCSMap cs) ->
-    size_valid (mk_cs (Map.remove a (HCSMap cs)) (HCSMaxCount cs) (HCSCount cs) (HCSEvict cs)).
+    ~ Map.In a (CSMap cs) ->
+    size_valid (mk_cs (Map.remove a (CSMap cs)) (CSMaxCount cs) (CSCount cs) (CSEvict cs)).
   Proof.
     unfold size_valid in *; intuition simpl.
     rewrite Map.cardinal_1 in *.
@@ -147,8 +208,8 @@ Lemma addr_clean_cachepred_remove :
 
   Lemma size_valid_remove_cardinal_ok : forall cs a,
     size_valid cs ->
-    Map.In a (HCSMap cs) ->
-    Map.cardinal (Map.remove a (HCSMap cs)) < HCSMaxCount cs.
+    Map.In a (CSMap cs) ->
+    Map.cardinal (Map.remove a (CSMap cs)) < CSMaxCount cs.
   Proof.
     unfold size_valid; intros.
     rewrite map_remove_cardinal.
@@ -198,19 +259,19 @@ Lemma addr_clean_cachepred_remove :
 
   Lemma size_valid_add :
     forall cs evictor vv a,
-    cardinal (HCSMap cs) < HCSMaxCount cs ->
-    Map.find a (HCSMap cs) = None ->
+    cardinal (CSMap cs) < CSMaxCount cs ->
+    Map.find a (CSMap cs) = None ->
     size_valid cs ->
-    size_valid (mk_cs (add a vv (HCSMap cs)) (HCSMaxCount cs) (HCSCount cs + 1) evictor).
+    size_valid (mk_cs (add a vv (CSMap cs)) (CSMaxCount cs) (CSCount cs + 1) evictor).
   Proof.
     unfold size_valid; intuition; simpl.
 
-    destruct (find a0 (HCSMap cs)) eqn:?; try congruence.
+    destruct (find a0 (CSMap cs)) eqn:?; try congruence.
     rewrite map_add_cardinal. omega.
     intuition repeat deex.
     apply MapFacts.find_mapsto_iff in H3; congruence.
 
-    destruct (Map.find a0 (HCSMap cs)) eqn:?.
+    destruct (Map.find a0 (CSMap cs)) eqn:?.
     rewrite map_add_dup_cardinal; auto.
     eexists; eapply MapFacts.find_mapsto_iff; eauto.
     rewrite map_add_cardinal. omega.
@@ -234,8 +295,8 @@ Lemma addr_clean_cachepred_remove :
     forall csmap d a tb bm h,
       d a = Some tb ->
       bm h = None ->
-     mem_pred (HighAEQ:= addr_eq_dec) (cachepred csmap bm) (mem_except d a) ✶ a |-> tb =p=>
-     mem_pred (HighAEQ:= addr_eq_dec) (cachepred (Map.add a (h, false) csmap) (upd bm h tb)) d.
+     mem_pred (HighAEQ:= addr_eq_dec) (cachepred csmap bm) (mem_except d a) ✶ a |+> tb =p=>
+     mem_pred (HighAEQ:= addr_eq_dec) (cachepred (Map.add a (h, false) csmap) (upd bm h (fst tb))) d.
   Proof.
     intros.
     eapply pimpl_trans; [ | apply mem_pred_absorb_nop; eauto ].
@@ -260,9 +321,343 @@ Lemma rep_none_upd_pimpl:
 Proof.
   unfold rep, cachepred; intros; cancel.
   eapply mem_pred_pimpl; intros.
-  destruct (find a (HCSMap cs)); [| cancel];
+  destruct (find a (CSMap cs)); [| cancel];
   destruct p; destruct b;
   cancel;
   destruct (Nat.eq_dec h0 h); subst;
   try congruence; rewrite upd_ne; auto.
 Qed.
+
+  Lemma size_valid_add_in : forall cs evictor vv v a,
+    Map.find a (CSMap cs) = Some v ->
+    size_valid cs ->
+    size_valid (mk_cs (Map.add a vv (CSMap cs)) (CSMaxCount cs) (CSCount cs) evictor).
+  Proof.
+    unfold size_valid; intuition; simpl.
+    rewrite map_add_dup_cardinal; auto.
+    eexists; eapply MapFacts.find_mapsto_iff; eauto.
+    rewrite map_add_dup_cardinal; auto.
+    eexists; eapply MapFacts.find_mapsto_iff; eauto.
+  Qed.
+
+  Lemma addr_valid_upd : forall a vs d cm,
+    addr_valid d cm ->
+    addr_valid (upd d a vs) cm.
+  Proof.
+    unfold addr_valid; intros.
+    destruct (addr_eq_dec a a0); subst.
+    rewrite upd_eq; congruence.
+    rewrite upd_ne; auto.
+  Qed.
+
+  Lemma addr_valid_upd_add : forall a vs vc d cm,
+    addr_valid d cm ->
+    addr_valid (upd d a vs) (Map.add a vc cm).
+  Proof.
+    intros.
+    eapply addr_valid_add; eauto.
+    apply upd_eq; auto.
+    apply addr_valid_upd; auto.
+  Qed.
+
+
+  Lemma incl_vsmerge_in : forall w v0 l l',
+    incl l (vsmerge (w, (vsmerge (v0, l')))) ->
+    List.In v0 (vsmerge (w, l')) ->
+    incl l (vsmerge (w, l')).
+  Proof.
+    unfold vsmerge, incl; simpl; intuition subst.
+    specialize (H _ H0); intuition.
+    specialize (H _ H0); intuition subst; auto.
+  Qed.
+
+  Lemma incl_vsmerge_in' : forall w v0 l l',
+    incl l (vsmerge (w, (vsmerge (v0, l')))) ->
+    List.In v0 l' ->
+    incl l (vsmerge (w, l')).
+  Proof.
+    unfold vsmerge, incl; simpl; intuition subst.
+    specialize (H _ H1); intuition subst.
+    right; auto.
+  Qed.
+
+  Lemma incl_vsmerge_in'' : forall a v l,
+    List.In v l ->
+    incl a (vsmerge (v, l)) ->
+    incl a l.
+  Proof.
+    unfold vsmerge, incl; intuition simpl in *.
+    specialize (H0 _ H1); intuition subst; auto.
+  Qed.
+
+Hint Resolve incl_vsmerge_in incl_vsmerge_in' incl_vsmerge_in''.
+
+  Lemma in_vsmerge_hd : forall w l,
+    List.In w (vsmerge (w, l)).
+  Proof.
+    unfold vsmerge; intuition.
+  Qed.
+
+  Lemma in_incl_trans: forall A (a b : list A) x,
+    incl a b ->
+    List.In x a ->
+    List.In x b.
+  Proof.
+    unfold incl; intros.
+    specialize (H _ H0); auto.
+  Qed.
+
+  Lemma incl_vsmerge_trans: forall a v l l',
+    incl a (vsmerge (v, l')) ->
+    incl l' l ->
+    incl a (vsmerge (v, l)).
+  Proof.
+    unfold incl, vsmerge; simpl; intros.
+    specialize (H _ H1); intuition.
+  Qed.
+
+  Lemma incl_vsmerge_in_trans : forall a v l l',
+    List.In v l ->
+    incl l' l ->
+    incl a (vsmerge (v, l')) ->
+    incl a l.
+  Proof.
+    intros.
+    eapply incl_vsmerge_in''; eauto.
+    eapply incl_vsmerge_trans; eauto.
+  Qed.
+
+Hint Resolve in_vsmerge_hd incl_vsmerge_trans incl_vsmerge_in_trans.
+
+
+
+
+  Lemma cachepred_synpred : forall cm bm a vs,
+    cachepred cm bm a vs =p=> exists vs', synpred cm bm a vs' *
+      [[ fst vs' = fst vs /\ incl (snd vs') (snd vs) /\
+         (addr_clean cm a -> snd vs' = nil) ]].
+  Proof.
+    unfold cachepred, synpred, addr_clean; intros.
+    destruct (Map.find a cm) eqn:?.
+    destruct p, b; cancel; auto.
+    apply incl_cons; auto; apply incl_nil.
+    deex; congruence.
+    apply incl_nil.
+    cancel.
+    apply incl_nil.
+  Qed.
+
+  Definition avs_match (avs1 avs2 : addr * valuset)  : Prop :=
+    let '(a1, vs1) := avs1 in let '(a2, vs2) := avs2 in
+    a2 = a1 /\ (fst vs2 = fst vs1) /\ incl (snd vs2) (snd vs1).
+
+  Definition nil_if_clean cm (avs : addr * valuset)  : Prop :=
+    let '(a, vs) := avs in addr_clean cm a -> snd vs = nil.
+
+  Lemma listpred_cachepred_synpred : forall l cm bm,
+    listpred (fun av => cachepred cm bm (fst av) (snd av)) l =p=> exists l',
+    listpred (fun av => synpred cm bm (fst av) (snd av)) l' *
+    [[ Forall2 avs_match l l' /\ Forall (nil_if_clean cm) l' ]].
+  Proof.
+    induction l; simpl; intros.
+    cancel; simpl; auto.
+    rewrite cachepred_synpred, IHl.
+    safecancel.
+    eassign ((a_1, (t1, l1)) :: l'); simpl.
+    cancel.
+    constructor; auto.
+    unfold avs_match; simpl; intuition.
+    auto.
+  Qed.
+
+  Lemma avs_match_map_fst_eq : forall l l',
+    Forall2 avs_match l l' ->
+    List.map fst l' = List.map fst l.
+  Proof.
+    unfold avs_match; induction 1; simpl; auto.
+    f_equal; auto.
+    destruct x, y; intuition.
+  Qed.
+
+  Lemma avs2mem_mem_match : forall V l l',
+    List.map fst l' = List.map fst l ->
+    @mem_match _ V _ (avs2mem addr_eq_dec l) (avs2mem addr_eq_dec l').
+  Proof.
+    induction l; destruct l'; simpl; try congruence; intros; cbn.
+    cbv; intuition.
+    destruct a, p; simpl in *.
+    inversion H; subst.
+    apply mem_match_upd.
+    apply IHl; auto.
+  Qed.
+
+  Lemma addr_valid_mem_match : forall d d' cm,
+    mem_match d d' ->
+    addr_valid d cm ->
+    addr_valid d' cm.
+  Proof.
+    unfold addr_valid; intros.
+    specialize (H0 _ H1).
+    edestruct mem_match_cases with (a := a); eauto; intuition.
+    repeat deex; congruence.
+  Qed.
+
+  Lemma avs_match_addr_valid : forall l l' cm,
+    Forall2 avs_match l l' ->
+    addr_valid (avs2mem addr_eq_dec l) cm ->
+    addr_valid (avs2mem addr_eq_dec l') cm.
+  Proof.
+    intros.
+    eapply addr_valid_mem_match; eauto.
+    apply avs2mem_mem_match.
+    apply avs_match_map_fst_eq; auto.
+  Qed.
+
+  Lemma avs_match_addr_valid' : forall l l' cm,
+    Forall2 avs_match l' l ->
+    addr_valid (avs2mem addr_eq_dec l) cm ->
+    addr_valid (avs2mem addr_eq_dec l') cm.
+  Proof.
+    intros.
+    eapply addr_valid_mem_match; eauto.
+    apply avs2mem_mem_match.
+    apply eq_sym.
+    apply avs_match_map_fst_eq; auto.
+  Qed.
+
+  Lemma avs_match_possible_sync : forall l l',
+    Forall2 avs_match l l' ->
+    possible_sync (avs2mem addr_eq_dec l) (avs2mem addr_eq_dec l').
+  Proof.
+    unfold possible_sync; induction 1; intuition.
+    unfold avs_match in H.
+    specialize (IHForall2 a); destruct x, y; cbn.
+    destruct v, v0; intuition; simpl in *; subst; repeat deex.
+    - destruct (addr_eq_dec a n); subst.
+      repeat rewrite upd_eq; auto.
+      right; do 3 eexists; intuition.
+      repeat rewrite upd_ne; auto.
+    - destruct (addr_eq_dec a n); subst.
+      repeat rewrite upd_eq; auto.
+      right; do 3 eexists; intuition.
+      repeat rewrite upd_ne; auto.
+      right; do 3 eexists; intuition eauto.
+  Qed.
+
+  Lemma avs_match_sync_invariant : forall l l' F,
+    Forall2 avs_match l l' ->
+    sync_invariant F ->
+    F (avs2mem addr_eq_dec l) ->
+    F (avs2mem addr_eq_dec l').
+  Proof.
+    unfold sync_invariant; intros.
+    eapply H0; eauto.
+    apply avs_match_possible_sync; auto.
+  Qed.
+
+  Lemma synpred_cachepred_sync : forall vs cm bm a,
+    sync_xform (synpred cm bm a vs) =p=> cachepred cm bm a vs.
+  Proof.
+    unfold cachepred, synpred; intros.
+    rewrite sync_xform_exists_comm.
+    apply pimpl_exists_l; intro vs0.
+    rewrite sync_xform_sep_star_dist.
+    destruct vs0 as [v0 l0].
+    destruct (Map.find a cm) eqn:?; try destruct p, b.
+    rewrite sync_xform_exists_comm; unfold pimpl; intros.
+    destruct_lift H.
+    rewrite sync_xform_sep_star_dist in H.
+    repeat rewrite sync_xform_lift_empty in H;
+    rewrite sync_xform_ptsto_subset_precise in H.
+    destruct_lift H; cleanup.
+    pred_apply; cancel.
+    unfold ptsto_subset; cancel; subst.
+
+    rewrite sync_xform_sep_star_dist.
+    repeat rewrite sync_xform_lift_empty.
+    rewrite sync_xform_ptsto_subset_precise.
+    unfold ptsto_subset; cancel; subst.
+    rewrite sync_xform_lift_empty.
+    rewrite sync_xform_ptsto_subset_precise.
+    unfold ptsto_subset; cancel; subst.
+  Qed.
+  
+  Lemma sync_xform_listpred_synpred_cachepred : forall l cm bm,
+    sync_xform (listpred (fun x => synpred cm bm (fst x) (snd x)) l) =p=>
+    listpred (fun x => cachepred cm bm (fst x) (snd x)) l.
+  Proof.
+    intros; rewrite sync_xform_listpred'; eauto.
+    intros; eapply synpred_cachepred_sync.
+  Qed.
+  
+  Lemma rep_synrep_split : forall cs (d: tagged_disk) bm F,
+    rep cs d bm /\ (exists d', synrep' cs d' bm * [[ F d' ]]) =p=>
+    (exists d', (rep cs d bm ⋀ synrep' cs d' bm) * [[ F d' ]]).
+  Proof.
+    intros.
+    rewrite pimpl_and_r_exists.
+    unfold pimpl; intros. destruct H. destruct H. destruct_lift H0.
+    exists x.
+    eapply sep_star_lift_apply'; eauto.
+    split; eauto.
+  Qed.
+
+  Lemma synrep_rep : forall cs d0 d bm,
+    synrep cs d0 d bm =p=> rep cs d0 bm.
+  Proof.
+    unfold synrep; intros.
+    apply pimpl_l_and; eauto.
+  Qed.
+
+
+  Lemma nil_if_clean_synced : forall l a cm vs,
+    Forall (nil_if_clean cm) l ->
+    addr_clean cm a ->
+    avs2mem addr_eq_dec l a = Some vs ->
+    NoDup (List.map fst l) ->
+    snd vs = nil.
+  Proof.
+    induction l; simpl; intros.
+    cbv in H1; congruence.
+    inversion H; inversion H2; subst.
+    destruct a; cbn in H1; simpl in *.
+    destruct (addr_eq_dec n a0); subst.
+    rewrite upd_eq in H1 by auto; inversion H1; subst; eauto.
+    rewrite upd_ne in H1 by auto.
+    eapply IHl; eauto; simpl in *.
+  Qed.
+
+
+  Lemma rep_synrep : forall (F : rawpred) d0 cs bm,
+    F d0 ->
+    sync_invariant F ->
+    rep cs d0 bm =p=> exists d, synrep cs d0 d bm * 
+      [[ F d /\ forall a vs, addr_clean (CSMap cs) a -> d a = Some vs -> snd vs = nil ]].
+  Proof.
+    unfold synrep; intros.
+    rewrite <- rep_synrep_split.
+    apply pimpl_and_split; auto.
+    unfold rep, synrep', mem_pred, mem_pred_one.
+    norml; unfold stars; simpl.
+    rewrite listpred_cachepred_synpred.
+    cancel.
+    eapply addr_valid_mem_match; eauto.
+    apply avs2mem_mem_match.
+    erewrite avs_match_map_fst_eq; eauto.
+    erewrite avs_match_map_fst_eq; eauto.
+    eapply avs_match_sync_invariant; eauto.
+    eapply nil_if_clean_synced; eauto.
+    erewrite avs_match_map_fst_eq; eauto.
+  Qed.
+
+  Lemma sync_invariant_sync_xform:
+  forall P,
+    sync_invariant (sync_xform P).
+Proof.
+  unfold sync_xform, sync_invariant; simpl; intros.
+  cleanup.
+  exists x.
+  intuition; apply possible_sync_after_sync; auto.
+Qed.
+
+Hint Resolve sync_invariant_sync_xform.
