src/PermCacheSec.v
@@ -1,0 +1,703 @@
+Require Import List.
+Require Import FMapAVL.
+Require Import FMapFacts.
+Require Import Word.
+Require Import Array.
+Require Import Pred.
+Require Import WordAuto.
+Require Import Omega.
+Require Import ListUtils.
+Require Import OrderedTypeEx.
+Require Import Arith.
+Require Import MapUtils.
+Require Import MemPred.
+Require Import ListPred.
+Require Import FunctionalExtensionality.
+Require Import ADestructPair DestructVarname.
+Require Export PermCacheLemmas.
+
+
+Import AddrMap.
+Import Map MapFacts.
+Import ListNotations.
+
+Set Implicit Arguments.
+
+  Theorem writeback_ok' :
+    forall a cs,
+    {< vs0,
+    PERM: None                       
+    PRE:bm
+        a |+> vs0 * [[ forall hb, Map.find a (CSMap cs) = Some hb -> exists v, bm (fst hb) = Some v ]]
+    POST:bm' RET:cs'
+      [[ bm' = bm ]] *
+      exists h v,
+      ([[ Map.find a (CSMap cs) = Some (h, true) /\ bm' h = Some v /\
+          cs' = mk_cs (Map.add a (h, false) (CSMap cs))
+                      (CSMaxCount cs) (CSCount cs) (CSEvict cs) ]] *
+         a |+> (v, vsmerge vs0)) \/
+      ([[ (Map.find a (CSMap cs) = None \/
+           Map.find a (CSMap cs) = Some (h, false)) /\ cs' = cs ]] * a |+> vs0) 
+    CRASH:
+      a |+> vs0 \/ (exists v, a |+> (v, vsmerge vs0))
+    >} writeback a cs.
+  Proof.
+    unfold writeback; intros.
+    prestep.
+    norml.
+    edestruct H5; eauto; cleanup; simpl in *.
+    unfold stars; norm.
+    unfold stars; cancel.
+    eassign F_.
+    eassign (t0, l).
+    eassign (emp (AT:=addr)(AEQ:=addr_eq_dec)(V:=valuset)).
+    cancel.
+    intuition; eauto.
+    hoare.
+    cancel.
+    cancel.
+
+    norml.
+    edestruct H5; eauto; cleanup; simpl in *.
+    unfold stars; norm.
+    unfold stars; cancel.
+    norm.
+    unfold stars; cancel.
+    intuition; eauto.
+    intuition.
+    intuition; eauto.
+    hoare.
+    cancel.
+    cancel.
+
+    norm.
+    unfold stars; cancel.
+    rewrite sep_star_comm; eauto.
+    intuition; eauto.
+    hoare.
+    cancel.
+    cancel.
+  Qed.
+
+Theorem writeback_ok :
+  forall a cs,
+    {< d,
+     PERM: None
+     PRE: bm
+       rep cs d bm
+     POST: bm'
+       RET:cs'
+         rep cs' d bm' * [[ bm' = bm ]] *
+          [[ addr_clean (CSMap cs') a ]] * 
+          [[ In a (CSMap cs) -> In a (CSMap cs')]]
+     CRASH:
+       exists cs', rep cs' d bm
+    >} writeback a cs.
+Proof.
+  unfold writeback, rep, addr_valid; intros; cleanup.
+  destruct (find a (CSMap cs)) eqn:D.
+  {
+    destruct p.
+    destruct b.
+    {
+      prestep. (* step not smart enough *)
+      unfold pimpl; intros m Hp; destruct_lift Hp.
+      assert (A: In a (CSMap cs)). {        
+        apply MapFacts.in_find_iff.
+        intuition; congruence.
+      }
+      specialize (H7 _ A) as Hx.
+      destruct (dummy0 a) eqn: D0; try congruence; clear Hx.
+      rewrite mem_pred_extract' in H; eauto.
+      unfold mem_pred_one, cachepred in H; simpl in H.
+      rewrite D in H.
+      destruct_lift H.
+
+      pred_apply; norm.
+      unfold stars; simpl; cancel.
+      Existential 3 := dummy.
+      Existential 5 := (dummy1, l).
+      cancel.
+      intuition; eauto.
+
+      step.
+      step; eauto.
+      erewrite <- mem_pred_absorb_nop with (hm:= dummy0)(a:= a); eauto.
+      unfold cachepred; simpl; eauto.
+      rewrite MapFacts.add_eq_o; eauto; simpl.
+      erewrite ptsto_subset_pimpl.
+      Existential 10:= l.
+      simpl; cancel; eauto.
+      apply mem_pred_pimpl_except; intros.
+      rewrite MapFacts.add_neq_o; auto.
+      unfold vsmerge; simpl.
+      eapply incl_cons; eauto.
+      apply incl_refl.
+
+      unfold size_valid in *; simpl; auto.
+      repeat rewrite map_add_dup_cardinal; auto.      
+      destruct (Nat.eq_dec a a0); subst; try congruence.
+      apply add_neq_in_iff in H0; eauto.
+      unfold addr_clean.
+      right; eexists; apply add_eq_o; eauto.
+      apply add_in_iff; intuition.
+
+      { (* Crash 1 *)
+        unfold pimpl; intros; apply H2;
+        pred_apply; cancel.
+        Existential 4 := {| CSMap := add a (h, false) (CSMap cs);
+                            CSMaxCount := CSMaxCount cs;
+                            CSCount := CSCount cs;
+                            CSEvict := CSEvict cs |}.
+        simpl; erewrite <- mem_pred_absorb_nop with (hm:= dummy0)(a:= a); eauto.
+        unfold cachepred; simpl; eauto.
+        rewrite MapFacts.add_eq_o; eauto; simpl.
+        erewrite ptsto_subset_pimpl.
+        Existential 7:= l.
+        simpl; cancel; eauto.
+        apply mem_pred_pimpl_except; intros.
+        rewrite MapFacts.add_neq_o; auto.
+        unfold vsmerge; simpl.
+        eapply incl_cons; eauto.
+        apply incl_refl.
+
+        unfold size_valid in *; simpl; auto.
+        repeat rewrite map_add_dup_cardinal; auto.      
+        simpl in *; destruct (Nat.eq_dec a a0); subst; try congruence.
+        apply add_neq_in_iff in H1; eauto.
+      }
+      {
+        apply H2;
+        pred_apply; cancel; eauto.
+        erewrite <- mem_pred_absorb_nop with (hm:= dummy0)(a:= a); eauto.
+        unfold cachepred; simpl; eauto.
+        rewrite D; cancel; eauto.
+      }
+    }    
+    unfold addr_clean; hoare.
+  }
+  unfold addr_clean; hoare.
+Qed.
+
+Hint Extern 1 (corr2 _ _ (Bind (writeback _ _) _)) => apply writeback_ok : prog.
+
+Hint Extern 0 (okToUnify (rep _ _ _) (rep _ _ _)) => constructor : okToUnify.
+Hint Extern 0 (okToUnify (synrep _ _ _ _ _) (synrep _ _ _ _ _)) => constructor : okToUnify.
+Hint Extern 0 (okToUnify (mem_pred ?p _) (mem_pred ?p _)) => constructor : okToUnify.
+
+
+Theorem evict_ok :
+  forall a cs,
+    {< d ,
+     PERM: None
+     PRE: bm
+      rep cs d bm
+    POST: bm'
+      RET:cs'
+        rep cs' d bm' * [[ bm' = bm ]] *
+        [[ ~ In a (CSMap cs') ]] *
+        [[ In a (CSMap cs) -> cardinal (CSMap cs') < CSMaxCount cs' ]]
+    CRASH:
+       exists cs', rep cs' d bm
+    >} evict a cs.
+  Proof.
+    unfold evict; step.
+    unfold rep in *; destruct (find a (CSMap r_)) eqn:D.
+    {
+      hoare.
+      eapply addr_valid_ptsto_subset in D as Hx;
+      eauto; cleanup.      
+      eapply addr_clean_cachepred_remove; eauto.
+      
+      apply size_valid_remove; auto.
+      eapply in_find_iff; intuition; congruence.
+      apply addr_valid_remove; auto.
+      eapply remove_1; eauto.
+      eapply size_valid_remove_cardinal_ok; eauto.
+    }
+    
+    {
+      hoare.    
+      eapply addr_clean_cachepred_remove_none; eauto.
+      apply size_valid_remove_notin; auto.
+      unfold not; intros.
+      eapply in_find_iff in D; congruence.
+      apply addr_valid_remove; auto.
+      eapply remove_1; eauto.
+      eapply size_valid_remove_cardinal_ok; eauto.
+    }
+Qed.
+
+Hint Extern 1 (corr2 _ _ (Bind (evict _ _) _)) => apply evict_ok : prog.
+
+
+
+Theorem maybe_evict_ok :
+  forall cs,
+  {< d,
+    PERM: None                          
+    PRE: bm
+      rep cs d bm
+    POST: bm' RET:cs'
+      rep cs' d bm'* [[ bm' = bm ]] *
+      [[ cardinal (CSMap cs') < CSMaxCount cs' ]]
+    CRASH:
+        exists cs', rep cs' d bm
+    >} maybe_evict cs.
+Proof.
+  unfold maybe_evict; step; step_r.
+  unfold rep, size_valid in *; destruct_lift H; cleanup; auto.
+  apply H8; apply in_find_iff; intuition; congruence.
+  unfold rep, size_valid in *; destruct_lift H; cleanup; auto.
+  rewrite cardinal_1 in *; cleanup; rewrite Heql in *; simpl in *; omega.
+  apply find_elements_hd in Heql;
+  apply H8; apply in_find_iff; intuition; congruence.  
+Qed.
+
+Hint Extern 1 (corr2 _ _ (Bind (maybe_evict _) _)) => apply maybe_evict_ok : prog.
+
+
+Theorem read_ok :
+  forall cs a,
+  {< d F tbs,
+    PERM: None                 
+    PRE: bm
+      rep cs d bm *
+      [[ (sep_star (AEQ:= addr_eq_dec) F (a |+> tbs))%pred d ]]
+    POST: bm' (RET:^(cs', r)
+      rep cs' d bm' * [[ bm' = upd bm r (fst tbs) ]])%pred
+    CRASH:
+      exists cs', rep cs' d bm
+  >} read a cs.
+Proof.
+  unfold read; intros.
+  safestep; eauto.
+  eapply ptsto_subset_valid' in H4 as Hx; cleanup; simpl in *.
+  repeat destruct_branch.
+  eapply pimpl_ok2. eapply ret_secure. safecancel; eauto.
+  step_r.
+  unfold rep in *; erewrite mem_pred_extract with (a := a) in H5; eauto; 
+  unfold cachepred at 2 in H5; rewrite Heqo in H5.
+  destruct b; destruct_lift H5;
+  symmetry; eapply upd_nop; eauto.
+  cancel; eauto.  
+
+  safestep.
+  unfold rep in *; erewrite mem_pred_extract with (a := a); eauto; 
+  unfold cachepred at 2; rewrite Heqo.
+  eassign (t0, x).
+  eassign F_.
+  eassign ([[ size_valid r_ ]] *
+                   [[ addr_valid d (CSMap r_) ]] *
+                   mem_pred (HighAEQ:=addr_eq_dec)
+                            (cachepred (CSMap r_) bm) (mem_except d a))%pred.
+  cancel.
+  eauto.
+  unfold rep in *; hoare.
+  
+  rewrite sep_star_comm.
+  eapply mem_pred_cachepred_add_absorb_clean; eauto.
+  apply size_valid_add; auto.
+  eapply addr_valid_add; eauto.
+  (eapply pimpl_trans; [ | apply mem_pred_absorb_nop; eauto]);
+  unfold cachepred at 3; rewrite Heqo;
+  cancel; eauto.
+  cancel.
+  unfold rep; cancel; eauto.
+  (eapply pimpl_trans; [ | apply mem_pred_absorb_nop; eauto]);
+  unfold cachepred at 3; rewrite Heqo;
+  cancel; eauto.
+Qed.
+
+Hint Extern 1 (corr2 _ _ (Bind (read _ _) _)) => apply read_ok : prog.
+
+Theorem write_ok:
+  forall cs a h,
+    {< d F tb0 tb,
+     PERM: None
+     PRE: bm
+            rep cs d bm *
+            [[ bm h = Some tb ]] *
+            [[ (F * a |+> tb0)%pred d ]]
+    POST: bm' RET:cs'
+      exists d',
+        rep cs' d' bm' * [[ bm' = bm ]] *
+        [[ (sep_star (AEQ:= addr_eq_dec) F  (a |+> (tb, vsmerge tb0)))%pred d' ]]
+    CRASH:
+      exists cs', rep cs' d bm    
+     >} write a h cs.
+Proof.
+    unfold write; intros.
+    safestep; eauto.
+    
+    eapply ptsto_subset_valid' in H0 as Hx; cleanup; simpl in *.
+    hoare.
+    {
+      unfold rep; simpl;
+      erewrite mem_pred_extract with (a := a) at 1; eauto.
+      unfold cachepred at 2; rewrite Heqo; eauto; cancel.
+      (rewrite mem_pred_pimpl_except;
+       [ | intros; apply cachepred_add_invariant with (v':=(h, true)); eassumption]).
+      rewrite <- mem_pred_absorb with (hm := d) (a := a);
+      unfold cachepred at 3;
+      rewrite MapFacts.add_eq_o by reflexivity.
+      destruct p_2.
+      cancel.
+      Existential 7:= (tb, vsmerge(t0, l)).
+      erewrite ptsto_subset_pimpl; eauto.
+      simpl; apply incl_tl; auto.
+      simpl; auto.
+      simpl; right; eapply In_incl; eauto.
+
+      cancel.
+      erewrite ptsto_subset_pimpl; eauto.
+      simpl; apply incl_tl; auto.
+      
+      eapply size_valid_add_in; eauto.
+      eapply addr_valid_upd_add; eauto.
+    }
+    eapply ptsto_subset_upd; eauto; apply incl_refl.
+    
+    {
+      unfold rep; simpl;
+      erewrite mem_pred_extract with (a := a) at 1; eauto.
+      unfold cachepred at 2; rewrite Heqo; eauto; cancel.
+      (rewrite mem_pred_pimpl_except;
+       [ | intros; apply cachepred_add_invariant with (v':=(h, true)); eassumption]).
+      rewrite <- mem_pred_absorb with (hm := d) (a := a);
+      unfold cachepred at 3;
+      rewrite MapFacts.add_eq_o by reflexivity.
+      cancel.
+      Existential 4:= (tb, vsmerge(t0, l)).
+      erewrite ptsto_subset_pimpl; eauto.
+      simpl; apply incl_tl; auto.
+      simpl; auto.
+      simpl; auto.
+
+      eapply size_valid_add; eauto.
+      eapply addr_valid_upd_add; eauto.
+    }
+    eapply ptsto_subset_upd; eauto; apply incl_refl.
+Qed.    
+
+Hint Extern 1 (corr2 _ _ (Bind (write _ _ _) _)) => apply write_ok : prog.
+
+Theorem begin_sync_ok :
+  forall cs,
+    {< d F,
+     PERM: None   
+     PRE:bm
+       rep cs d bm * [[ F d /\ sync_invariant F ]]
+     POST:bm' RET:cs
+       exists d',
+         synrep cs d d' bm * [[ bm' = bm ]] * [[ F d' ]]
+     CRASH:
+       exists cs', rep cs' d bm
+    >} begin_sync cs.
+  Proof.
+    unfold begin_sync, synrep.
+    step.
+    prestep.
+    norml; unfold stars; simpl.
+    rewrite rep_synrep by eauto.
+    cancel; eauto.
+  Qed.
+  
+Theorem end_sync_ok :
+  forall cs,
+   {< d0 d,
+    PERM: None
+    PRE:bm
+      synrep cs d0 d bm
+    POST:bm' RET:cs
+      rep cs d bm' * [[ bm' = bm ]]
+    CRASH:
+      exists cs', rep cs' d0 bm
+    >} end_sync cs.
+  Proof.
+    unfold end_sync; intros.
+    safestep.
+    eassign (fun x => synrep cs (fst x) (fst (snd x)) (snd (snd x))).
+    eassign F_.
+    eassign (d0, (d, bm)).
+    simpl; cancel; eauto.
+    simpl; auto.
+    auto.
+    step.
+    step.
+    
+    unfold rep, synrep, synrep', mem_pred, mem_pred_one; simpl.
+    rewrite sync_xform_and_dist. rewrite pimpl_r_and.
+    repeat (rewrite sync_xform_sep_star_dist || rewrite sync_xform_lift_empty || rewrite sync_xform_exists_comm).
+    norml; unfold stars; simpl.
+    repeat (rewrite sync_xform_sep_star_dist || rewrite sync_xform_lift_empty || rewrite sync_xform_exists_comm).
+    cancel; auto.
+    rewrite sync_xform_listpred_synpred_cachepred; auto.
+    rewrite sync_xform_sync_invariant by auto.
+    apply synrep_rep.
+    simpl; cancel.
+    apply synrep_rep.
+  Qed.
+
+  
+  Theorem sync_ok' :
+    forall cs a,
+   {< d0 d (F F' : rawpred) v0 v',
+    PERM: None   
+    PRE:bm
+      synrep cs d0 d bm * [[ sync_invariant F ]] *
+      [[ (F * a |+> v0)%pred d ]] *
+      [[ (F' * a |+> v')%pred d0 ]]
+    POST:bm' RET:cs
+      exists d,
+        synrep cs d0 d bm' * [[ bm' = bm ]] *
+        [[ (F * a |+> (fst v0, nil))%pred d ]]
+    CRASH:
+      exists cs', rep cs' d0 bm
+    >} sync a cs.
+  Proof.
+    unfold sync; intros.
+    eapply pimpl_ok2; monad_simpl. apply writeback_ok'.
+    intros.
+    norml; unfold stars; simpl.
+    denote (_ d) as Hx; apply ptsto_subset_valid' in Hx as Hy; repeat deex.
+    denote (_ d0) as Hz; apply ptsto_subset_valid' in Hz as Hy; repeat deex.
+    unfold synrep, rep, synrep'.
+    rewrite sep_star_lift_empty.
+    rewrite sep_star_lift_empty.
+    rewrite lift_empty_and_distr_l; norml; unfold stars; simpl.
+    rewrite mem_pred_extract with (a := a) (hm := d) by eauto.
+    rewrite mem_pred_extract with (a := a) (hm := d0) by eauto.
+    unfold cachepred at 2; unfold synpred at 2; simpl in *.
+    destruct (Map.find a (CSMap cs)) eqn:?; try destruct p, b.
+    - unfold ptsto_subset.
+      repeat (rewrite pimpl_exists_l_star_r ||
+              rewrite pimpl_exists_r_star_r ||
+              rewrite pimpl_and_l_exists ||
+              rewrite pimpl_and_r_exists ||
+              apply pimpl_exists_l; intros ).
+      setoid_rewrite sep_star_assoc at 2.
+      repeat rewrite sep_star_lift_empty.
+      setoid_rewrite sep_star_assoc at 2.
+      repeat rewrite sep_star_lift_empty.
+      setoid_rewrite sep_star_assoc at 2.
+      repeat rewrite sep_star_lift_empty.
+      setoid_rewrite <- sep_star_assoc at 1 2.
+      rewrite lift_empty_and_distr_r.
+      norml; unfold stars; simpl; subst.
+      rewrite sep_star_ptsto_and_eq.
+      safecancel; simpl in *; cleanup.
+      eassign (t2, x3).
+      eassign x3.
+      cancel; simpl; eauto.
+      simpl; apply incl_refl.
+      auto.
+
+      step.
+      step.
+      repeat cleanup.
+      2: eapply ptsto_subset_upd with (vs' := nil); eauto; apply incl_refl.
+      rewrite sep_star_and_distr; unfold synrep.
+      apply pimpl_and_split.
+      + rewrite pimpl_l_and; unfold rep; cancel.
+        erewrite <- upd_nop with (m := d0) at 2 by eauto.
+        rewrite <- mem_pred_absorb with (hm := d0) (a := a).
+        unfold cachepred at 3.
+        rewrite MapFacts.add_eq_o by reflexivity.
+        unfold ptsto_subset; cancel; eauto.
+        rewrite mem_pred_pimpl_except.
+        2: intros; apply cachepred_add_invariant; eassumption.
+        cancel.        
+        eapply size_valid_add_in; eauto.
+        eapply addr_valid_add; eauto.
+      + rewrite pimpl_r_and; unfold synrep'; cancel.
+        rewrite <- mem_pred_absorb with (hm := d) (a := a).
+        unfold synpred at 3.
+        rewrite MapFacts.add_eq_o by reflexivity.
+        unfold ptsto_subset; cancel; eauto.
+        rewrite mem_pred_pimpl_except.
+        2: intros; apply synpred_add_invariant; eassumption.
+        eassign (a1, old); simpl.
+        cancel.
+        simpl; auto.
+        simpl; auto.
+        eapply size_valid_add_in; eauto.
+        eapply addr_valid_add; eauto.
+        rewrite upd_eq; auto.
+        apply addr_valid_upd; auto.
+      + (* crash *)
+        cancel.
+        repeat cleanup.
+        rewrite sep_star_and_distr, pimpl_l_and.
+        unfold rep; cancel; eauto.
+        repeat cleanup.
+        eapply pimpl_trans; [ | apply mem_pred_absorb_nop; eauto ].
+        unfold cachepred at 3; rewrite Heqo.
+        repeat cleanup.
+        unfold ptsto_subset; cancel; eauto.
+        repeat cleanup.
+        eapply incl_tran; eauto.
+        unfold vsmerge; simpl; auto.
+        apply incl_cons; eauto.
+
+    - unfold ptsto_subset.
+      repeat (rewrite pimpl_exists_l_star_r ||
+              rewrite pimpl_exists_r_star_r ||
+              rewrite pimpl_and_l_exists ||
+              rewrite pimpl_and_r_exists ||
+              apply pimpl_exists_l; intros ).
+      setoid_rewrite sep_star_assoc at 2.
+      rewrite sep_star_lift_empty.
+      setoid_rewrite sep_star_assoc at 2.
+      rewrite sep_star_lift_empty.
+      setoid_rewrite <- sep_star_assoc at 1 2.
+      rewrite lift_empty_and_distr_r.
+      norml; unfold stars; simpl; subst.
+      rewrite sep_star_ptsto_and_eq.
+      cancel; subst; eauto.
+
+      prestep; norml; unfold stars; simpl;
+      intuition; repeat deex; try congruence; inv_option_eq.
+      cancel.
+      2: eapply ptsto_subset_upd with (vs' := nil); eauto; apply incl_refl.
+      rewrite sep_star_and_distr; unfold synrep.
+      apply pimpl_and_split.
+      + rewrite pimpl_l_and; unfold rep; cancel.
+        erewrite <- upd_nop with (m := d0) at 2 by eauto.
+        rewrite <- mem_pred_absorb with (hm := d0) (a := a).
+        unfold cachepred at 3.
+        rewrite Heqo.
+        unfold ptsto_subset; cancel.
+        eapply incl_tran; eauto.
+      + rewrite pimpl_r_and; unfold synrep'; cancel.
+        rewrite <- mem_pred_absorb with (hm := d) (a := a).
+        unfold synpred at 3.
+        rewrite Heqo.
+        unfold ptsto_subset; cancel; eauto.
+        apply addr_valid_upd; auto.
+      + (* crash *)
+        cancel.
+        rewrite sep_star_and_distr, pimpl_l_and.
+        unfold rep; cancel; eauto.
+        eapply pimpl_trans; [ | apply mem_pred_absorb_nop; eauto ].
+        unfold cachepred at 3; rewrite Heqo.
+        unfold ptsto_subset; cancel; eauto.
+        eapply incl_tran; eauto.
+
+    - unfold ptsto_subset.
+      repeat (rewrite pimpl_exists_l_star_r ||
+              rewrite pimpl_exists_r_star_r ||
+              rewrite pimpl_and_l_exists ||
+              rewrite pimpl_and_r_exists ||
+              apply pimpl_exists_l; intros ).
+      setoid_rewrite sep_star_assoc at 2.
+      rewrite sep_star_lift_empty.
+      setoid_rewrite <- sep_star_assoc at 1 2.
+      rewrite lift_empty_and_distr_r.
+      norml; unfold stars; simpl; subst.
+      rewrite sep_star_ptsto_and_eq.
+      cancel; subst; eauto.
+
+      prestep; norml; unfold stars; simpl;
+      intuition; repeat deex; try congruence; inv_option_eq.
+      cancel.
+      2: eapply ptsto_subset_upd with (vs' := nil); eauto; apply incl_refl.
+      rewrite sep_star_and_distr; unfold synrep.
+      apply pimpl_and_split.
+      + rewrite pimpl_l_and; unfold rep; cancel.
+        erewrite <- upd_nop with (m := d0) at 2 by eauto.
+        rewrite <- mem_pred_absorb with (hm := d0) (a := a).
+        unfold cachepred at 3.
+        rewrite Heqo.
+        unfold ptsto_subset; cancel.
+        eapply incl_tran; eauto.
+      + rewrite pimpl_r_and; unfold synrep'; cancel.
+        rewrite <- mem_pred_absorb with (hm := d) (a := a).
+        unfold synpred at 3.
+        rewrite Heqo.
+        unfold ptsto_subset; cancel; eauto.
+        apply addr_valid_upd; auto.
+      + (* crash *)
+        cancel.
+        rewrite sep_star_and_distr, pimpl_l_and.
+        unfold rep; cancel; eauto.
+        eapply pimpl_trans; [ | apply mem_pred_absorb_nop; eauto ].
+        unfold cachepred at 3; rewrite Heqo.
+        unfold ptsto_subset; cancel; eauto.
+        eapply incl_tran; eauto.
+
+    Unshelve. all: eauto.
+  Qed.
+
+
+  Theorem sync_synrep_helper_1 : forall m cs d0 d a (F : @pred _ addr_eq_dec _) v,
+    synrep cs d0 d m ->
+    (F * a |+> v)%pred d ->
+    exists (F0 : @pred _ addr_eq_dec _) v0,
+    (F0 * a |+> v0)%pred d0.
+  Proof.
+    unfold synrep, rep, synrep', ptsto_subset; intros.
+    case_eq (d0 a); intros.
+    - destruct p.
+      eapply any_sep_star_ptsto in H1.
+      pred_apply.
+      safecancel.
+      eassign (w, l).
+      eassign l.
+      cancel.
+      firstorder.
+    - destruct H.
+      destruct_lift H.
+      destruct_lift H2.
+      destruct_lift H0.
+      apply ptsto_valid' in H0.
+      eapply mem_pred_absent_lm in H; eauto.
+      eapply mem_pred_absent_hm in H2; eauto.
+      congruence.
+
+      unfold synpred, ptsto_subset; intros.
+      destruct (Map.find a0 (CSMap cs)); try destruct p; try destruct b; cancel.
+
+      unfold cachepred, ptsto_subset; intros.
+      destruct (Map.find a0 (CSMap cs)); try destruct p; try destruct b; cancel.
+  Qed.
+
+  Theorem sync_synrep_helper_2 : forall cs d0 d a (F : @pred _ addr_eq_dec _) v,
+    (F * a |+> v)%pred d ->
+    synrep cs d0 d =p=> synrep cs d0 d * exists (F0 : @pred _ addr_eq_dec _) v0,
+    [[ (F0 * a |+> v0)%pred d0 ]].
+  Proof.
+    unfold pimpl; intros.
+    eapply sync_synrep_helper_1 in H; eauto; repeat deex.
+    pred_apply; cancel.
+  Qed.
+
+
+  Theorem sync_ok : forall cs a,
+    {< d0 d (F : rawpred) v0,
+    PRE:hm
+      synrep cs d0 d *
+      [[ (F * a |+> v0)%pred d ]] *
+      [[ sync_invariant F ]]
+    POST:hm' RET:cs exists d,
+      synrep cs d0 d *
+      [[ (F * a |+> (fst v0, nil))%pred d ]]
+    CRASH:hm'
+      exists cs', rep cs' d0
+    >} sync a cs.
+  Proof.
+    intros.
+    eapply pimpl_ok2; monad_simpl.
+    apply sync_ok'.
+    intros; norml; unfold stars; simpl.
+    rewrite sync_synrep_helper_2 by eauto.
+    safecancel.
+    eauto.
+    step.
+  Qed.
+
+
+  Hint Extern 1 ({{_}} Bind (read _ _) _) => apply read_ok : prog.
+  Hint Extern 1 ({{_}} Bind (sync _ _) _) => apply sync_ok : prog.
+  Hint Extern 1 ({{_}} Bind (begin_sync _) _) => apply begin_sync_ok : prog.
+  Hint Extern 1 ({{_}} Bind (end_sync _) _) => apply end_sync_ok : prog.
