src/PermInstr.v
@@ -51,16 +51,16 @@ Qed.
 
 Lemma read_secure:
   forall pr a,
-    {< tb tbs F,
+    {< tbs F,
        PERM: pr
        PRE: bm
-          (F * a|-> (tb, tbs))%pred
+          (F * a|+> tbs)%pred
        POST: bm'
           RET: i
-          (F * a|-> (tb, tbs) * [[ bm i = None ]] *
-           [[ bm' = upd (AEQ:= PeanoNat.Nat.eq_dec) bm i tb ]])%pred
+          (F * a|+> tbs * [[ bm i = None ]] *
+           [[ bm' = upd (AEQ:= PeanoNat.Nat.eq_dec) bm i (fst tbs) ]])%pred
        CRASH:
-         (F * a|->(tb, tbs))%pred
+         (F * a|+>tbs)%pred
      >} Read a.
 Proof.
   unfold corr2; intros.
@@ -71,7 +71,7 @@ Proof.
     inv_exec_perm.
     edestruct H4; eauto.
     pred_apply; cancel; eauto.
-    apply ptsto_valid' in H; cleanup; eauto.  
+    apply ptsto_subset_valid' in H; cleanup; eauto.  
     split; auto.
     clear H0; eapply bind_secure; intuition.  
     unfold permission_secure; intros.
@@ -84,7 +84,7 @@ Proof.
     inv_exec_perm; cleanup; auto.
     edestruct H4; eauto.
     pred_apply; cancel; eauto.
-    apply ptsto_valid' in H; cleanup; eauto.
+    apply ptsto_subset_valid' in H; cleanup; eauto.
   }
   split_ors; cleanup.
   {
@@ -101,7 +101,7 @@ Proof.
     inv_exec_perm; cleanup; auto.
     edestruct H4; eauto.
     pred_apply; cancel; eauto.
-    apply ptsto_valid' in H; cleanup; eauto.
+    apply ptsto_subset_valid' in H; cleanup; eauto.
   }
   {
     split.
@@ -109,7 +109,7 @@ Proof.
     inv_exec_perm.
     edestruct H4; eauto.
     pred_apply; cancel; eauto.
-    apply ptsto_valid' in H; cleanup; eauto.
+    apply ptsto_subset_valid' in H; cleanup; eauto.
     split_ors; cleanup; try congruence.
     eapply bind_secure; intuition.
     unfold permission_secure; intros.
@@ -120,7 +120,7 @@ Proof.
     inv_exec_perm; cleanup; auto.
     edestruct H4; eauto.
     pred_apply; cancel; eauto.
-    apply ptsto_valid' in H; cleanup; eauto.
+    apply ptsto_subset_valid' in H; cleanup; eauto.
   }
 Qed.
 
@@ -129,12 +129,12 @@ Lemma write_secure:
     {< F tb tbs,
        PERM: pr
        PRE: bm
-          (F * a|->tbs * [[ bm i = Some tb ]])%pred
+          (F * a|+>tbs * [[ bm i = Some tb ]])%pred
        POST: bm'
           RET: tt
-          (F * a|->(tb, vsmerge tbs) * [[ bm' = bm ]])%pred
+          (F * a|+>(tb, vsmerge tbs) * [[ bm' = bm ]])%pred
        CRASH:
-          (F * a|->tbs)%pred
+          (F * a|+>tbs)%pred
      >} Write a i.
 Proof.
   unfold corr2; intros.
@@ -144,9 +144,12 @@ Proof.
   {
     inv_exec_perm.
     edestruct H4; eauto.
-    apply ptsto_valid' in H as Hx; cleanup; eauto.
-    eapply ptsto_upd' with (v:= (tb, vsmerge tbs)) in H;
+    apply ptsto_subset_valid' in H as Hx; cleanup; eauto.
+    eapply ptsto_subset_upd  with (v:= tb)(vs':= vsmerge (fst dummy2, x0)) in H.
     pred_apply; cancel.
+    unfold vsmerge; simpl;
+    apply ListUtils.incl_cons2; auto.
+    
     split; eauto.
     
     clear H0; eapply bind_secure; intuition.
@@ -171,21 +174,23 @@ Proof.
     unfold permission_secure; intros.
     inv_exec_perm; cleanup; auto.
     edestruct H4; eauto.
-    apply ptsto_valid' in H as Hx; cleanup; eauto.
-    eapply ptsto_upd' with (v:= (tb, vsmerge tbs)) in H;
+    apply ptsto_subset_valid' in H as Hx; cleanup; eauto.
+    eapply ptsto_subset_upd  with (v:= tb)(vs':= vsmerge (fst dummy2, x)) in H.
     pred_apply; cancel.
+    unfold vsmerge; simpl;
+    apply ListUtils.incl_cons2; auto.
   }
   {
     split.
     right; eexists; intuition.
     inv_exec_perm.
     edestruct H4; eauto.
-    apply ptsto_valid' in H as Hx; cleanup; eauto.
-    eapply ptsto_upd' with (v:= (tb, vsmerge tbs)) in H;
+    apply ptsto_subset_valid' in H as Hx; cleanup; eauto.
+    eapply ptsto_subset_upd  with (v:= tb)(vs':= vsmerge (fst dummy2, x0)) in H as Hy.
     pred_apply; cancel.
-    apply ptsto_valid' in H; cleanup; eauto.
+    unfold vsmerge; simpl;
+    apply ListUtils.incl_cons2; auto.
     split_ors; cleanup; try congruence.
-    inversion H0; cleanup; eauto.
 
     eapply bind_secure; intuition.
     unfold permission_secure; intros.
@@ -195,9 +200,11 @@ Proof.
     unfold permission_secure; intros.
     inv_exec_perm; cleanup; auto.
     edestruct H4; eauto.
-    apply ptsto_valid' in H as Hx; cleanup; eauto.
-    eapply ptsto_upd' with (v:= (tb0, vsmerge tbs0)) in H;
+    apply ptsto_subset_valid' in H as Hx; cleanup; eauto.
+    eapply ptsto_subset_upd  with (v:= tb)(vs':= vsmerge (fst dummy2, x3)) in H.
     pred_apply; cancel.
+    unfold vsmerge; simpl;
+    apply ListUtils.incl_cons2; auto.
   }
 Qed.
 
@@ -413,6 +420,77 @@ Proof.
   }
 Qed.
 
+Lemma ret_secure':
+  forall A T P pr (v: T),
+     {< (e: A),
+       PERM: pr
+       PRE: bm
+         P e
+       POST: bm' RET : r
+         P e * [[ r = v ]] *
+         [[ bm' = bm ]]
+       CRASH:
+         P e
+     >} Ret v.
+Proof.
+  unfold corr2; intros.
+  destruct_lift H; cleanup.
+  repeat inv_exec_perm; simpl in *; cleanup.
+   destruct out; cleanup.
+  {
+    inv_exec_perm.
+    edestruct H4; eauto.
+    pred_apply; cancel; eauto.
+    split; auto.
+    clear H0; eapply bind_secure; intuition.  
+    unfold permission_secure; intros.
+    inv_exec_perm; cleanup; auto.
+    simpl; eauto.
+    simpl; eauto.
+    
+    unfold permission_secure; intros.
+    clear H1.
+    inv_exec_perm; cleanup; auto.
+    edestruct H4; eauto.
+    pred_apply; cancel; eauto.
+  }
+  split_ors; cleanup.
+  {
+    split.
+    right; eexists; intuition.
+    inv_exec_perm.
+    pred_apply; cancel.
+    eapply bind_secure; intuition.
+    unfold permission_secure; intros.
+    inv_exec_perm; cleanup; auto.
+    simpl; eauto.
+    simpl; eauto.
+    unfold permission_secure; intros.
+    inv_exec_perm; cleanup; auto.
+    edestruct H4; eauto.
+    pred_apply; cancel; eauto.
+  }
+  {
+    split.
+    right; eexists; intuition.
+    inv_exec_perm.
+    edestruct H4; eauto.
+    pred_apply; cancel; eauto.
+    split_ors; cleanup; try congruence.
+    eapply bind_secure; intuition.
+    unfold permission_secure; intros.
+    inv_exec_perm; cleanup; auto.
+    simpl; eauto.
+    simpl; eauto.
+    unfold permission_secure; intros.
+    inv_exec_perm; cleanup; auto.
+    edestruct H4; eauto.
+    pred_apply; cancel; eauto.
+  }
+Qed.
+
+
+
 (*
 Lemma exec_trace_irrelevance:
   forall T (p: prog T) pr tr tr' tr'' d bm r,
@@ -470,9 +548,109 @@ Proof.
 Qed.
 *)
 
+Lemma sync_invariant_sync_mem_apply:
+  forall (P: rawpred) m,
+    P m ->
+    sync_invariant P ->
+    P (sync_mem m).
+Proof.
+  unfold sync_invariant; intros.
+  eapply H0; eauto.
+  apply possible_sync_sync_mem.
+Qed.
+
+Lemma sync_secure:
+  forall A pr P,
+     {< (e: A),
+       PERM: pr
+       PRE: bm
+         P e * [[ sync_invariant (P e) ]]
+       POST: bm' RET : tt
+         sync_xform (P e) *
+         [[ bm' = bm ]]
+       CRASH:
+         P e
+     >} Sync.
+Proof.
+  unfold corr2; intros.
+  destruct_lift H; cleanup.
+  repeat inv_exec_perm; simpl in *; cleanup.
+   destruct out; cleanup.
+  {
+    inv_exec_perm.
+    edestruct H4; eauto.
+    rewrite <- sync_xform_sync_invariant with (p:= dummy); eauto;
+    repeat rewrite <- sep_star_assoc;
+    rewrite <- sync_xform_sep_star_dist.
+    repeat (apply sep_star_lift_apply'; eauto).
+    apply sync_xform_pred_apply; auto.
+    
+    split; auto.
+    clear H0; eapply bind_secure; intuition.  
+    unfold permission_secure; intros.
+    inv_exec_perm; cleanup; auto.
+    simpl; eauto.
+    simpl; eauto.
+    
+    unfold permission_secure; intros.
+    clear H1; inv_exec_perm; cleanup; auto.
+    edestruct H4; eauto.
+    rewrite <- sync_xform_sync_invariant with (p:= dummy); eauto;
+    repeat rewrite <- sep_star_assoc;
+    rewrite <- sync_xform_sep_star_dist.
+    repeat (apply sep_star_lift_apply'; eauto).
+    apply sync_xform_pred_apply; auto.
+  }
+  split_ors; cleanup.
+  {
+    split.
+    right; eexists; intuition.
+    inv_exec_perm.
+    pred_apply; cancel.
+    eapply bind_secure; intuition.
+    unfold permission_secure; intros.
+    inv_exec_perm; cleanup; auto.
+    simpl; eauto.
+    simpl; eauto.
+    unfold permission_secure; intros.
+    inv_exec_perm; cleanup; auto.
+    edestruct H4; eauto.
+    rewrite <- sync_xform_sync_invariant with (p:= dummy); eauto;
+    repeat rewrite <- sep_star_assoc;
+    rewrite <- sync_xform_sep_star_dist.
+    repeat (apply sep_star_lift_apply'; eauto).
+    apply sync_xform_pred_apply; auto.
+  }
+  {
+    split.
+    right; eexists; intuition.
+    inv_exec_perm.
+    edestruct H4; eauto.
+    rewrite <- sync_xform_sync_invariant with (p:= dummy); eauto;
+    repeat rewrite <- sep_star_assoc;
+    rewrite <- sync_xform_sep_star_dist.
+    repeat (apply sep_star_lift_apply'; eauto).
+    apply sync_xform_pred_apply; auto.
+    split_ors; cleanup; try congruence.
+    eapply bind_secure; intuition.
+    unfold permission_secure; intros.
+    inv_exec_perm; cleanup; auto.
+    simpl; eauto.
+    simpl; eauto.
+    unfold permission_secure; intros.
+    inv_exec_perm; cleanup; auto.
+    edestruct H4; eauto.
+    rewrite <- sync_xform_sync_invariant with (p:= dummy); eauto;
+    repeat rewrite <- sep_star_assoc;
+    rewrite <- sync_xform_sep_star_dist.
+    repeat (apply sep_star_lift_apply'; eauto).
+    apply sync_xform_pred_apply; auto.
+  }
+Qed.
 
 Hint Extern 1 (corr2 _ _ (Bind (Read _) _)) => apply read_secure : prog.
 Hint Extern 1 (corr2 _ _ (Bind (Write _ _) _)) => apply write_secure : prog.
 Hint Extern 1 (corr2 _ _ (Bind (Seal _ _) _)) => apply seal_secure : prog.
 Hint Extern 1 (corr2 _ _ (Bind (Unseal _) _)) => apply unseal_secure : prog.
-Hint Extern 1 (corr2 _ _ (Bind (Ret _) _)) => apply ret_secure : prog.
+Hint Extern 1 (corr2 _ _ (Bind Sync _)) => apply sync_secure : prog.
+Hint Extern 1 (corr2 _ _ (Bind (Ret _) _)) => apply ret_secure' : prog.
