src/PermPredCrash.v
@@ -4,6 +4,7 @@ Require Import List ListUtils.
 Require Import FunctionalExtensionality.
 Require Import Morphisms.
 Require Import Arith.
+Require Import ListPred MemPred.
 Require Export PermAsyncDisk.
 
 Set Implicit Arguments.
@@ -1317,6 +1318,7 @@ Proof.
   eapply possible_sync_possible_crash_trans; eauto.
 Qed.
 
+
 Hint Resolve sync_invariant_ptsto_subset.
 Hint Resolve sync_invariant_ptsto_any.
 Hint Resolve sync_invariant_ptsto_nil.
@@ -1328,6 +1330,25 @@ Hint Resolve sync_invariant_and.
 Hint Resolve sync_invariant_or.
 Hint Resolve sync_invariant_crash_xform.
 
+Theorem sync_invariant_listpred :
+  forall A (l: list A) f,
+    (forall a, sync_invariant (f a)) ->
+    sync_invariant (listpred f l).
+Proof.
+  induction l; simpl; eauto.
+Qed.
+
+Hint Resolve sync_invariant_listpred.
+
+Theorem sync_invariant_mem_pred :
+  forall A B AEQ (f: A -> B -> pred) (m: @Mem.mem A AEQ B),
+    (forall a b, sync_invariant (f a b)) ->
+    sync_invariant (mem_pred f m).
+Proof.
+  unfold mem_pred, mem_pred_one; intros; eauto.
+Qed.
+
+Hint Resolve sync_invariant_mem_pred.
 
 Theorem upd_sync_invariant : forall (p : @pred _ _ _) m a v l l',
   sync_invariant p ->
@@ -1384,4 +1405,30 @@ Proof.
   setoid_rewrite sep_star_comm.
   apply sep_star_assoc; apply sep_star_comm.
   apply sep_star_lift_apply'; eauto.
+Qed.
+
+Hint Resolve sync_invariant_listpred.
+
+Theorem sync_xform_listpred : forall V (l : list V) prd,
+  sync_xform (listpred prd l) <=p=> listpred (fun x => sync_xform (prd x)) l.
+Proof.
+  induction l; simpl; intros; split; auto.
+  apply sync_xform_emp.
+  apply sync_xform_emp.
+  rewrite sync_xform_sep_star_dist.
+  rewrite IHl; auto.
+  rewrite sync_xform_sep_star_dist.
+  rewrite IHl; auto.
+Qed.
+
+
+Lemma sync_xform_listpred' : forall T (l : list T) p q,
+  (forall x, sync_xform (p x) =p=> q x) ->
+  sync_xform (listpred p l) =p=> listpred q l.
+Proof.
+  induction l; simpl; intros; auto.
+  apply sync_xform_emp.
+  repeat rewrite sync_xform_sep_star_dist.
+  rewrite IHl by eauto.
+  rewrite H; auto.
 Qed.
